use the ctxr tactics to compose ctx_refines

cellio/CellioAll.v
@@ -18,31 +18,35 @@ Module CellioAll. Section CellioAll.
   Qed.
 
   Variable CtxA: SMod.t.
+  Variable CtxI: HMod.t.
+  Variable CtxInitCond : iProp Σ.
+  
   Local Definition smod_src : SMod.t := MainA.Mod ☆ CtxA.
-
   Local Definition sp : string → option fspec := sp_from smod_src.
-  Local Definition Ctx := Seal.sealing CRIS (SMod.to_hmod sp CtxA).
   Local Definition mod_cancel : HMod.t := SModCancel.to_hmod smod_src.
   Local Definition mod_src : HMod.t := SMod.to_hmod sp smod_src.
-  Local Definition mod_tgt : HMod.t := MainI.t ★ CellioI.t ★ Ctx.
+  Local Definition mod_tgt : HMod.t := MainI.t ★ CellioI.t ★ CtxI.
+  Local Definition with_trivial_spec body := {|fsb_fspec := fspec_trivial; fsb_body := body|}.
   
-  Local Definition main_fsp : fspec := fspec_trivial.
-  Local Definition CtxInitCond : iProp Σ := emp%I.
-  Local Definition init_cond : iProp Σ := MainA.InitCond ∗ CellioA.InitCond ∗ CtxInitCond.
-  
-  (* Apply cancellation to linked spec module *)
-  Lemma cancel_src :
-    refines (mod_cancel, (init_cond ∗ main_fsp.(precond) tt tt↑ tt↑)%I) 
-            (mod_src, init_cond).
-  Proof. eapply cancellation; try by econs. i. iIntros "%POST". iPureIntro. des; eauto. Qed.
-
-  Local Definition trivial_specbody body := {|fsb_fspec := fspec_trivial; fsb_body := body|}.
-
   Hypothesis ModulesWF : HMod.wf mod_tgt.
+  Hypothesis CtxCorrect: ctx_refines (SMod.to_hmod sp CtxA, CtxInitCond) (CtxI, emp%I).
   Hypothesis inputInCtx : ∃ msk sc input (SCP: incl sc CtxA.(SMod.scopes)),
-    alist_find CtxHdr.input (SMod.fnsems CtxA) = Some (msk, sc, trivial_specbody input).
+    alist_find CtxHdr.input (SMod.fnsems CtxA) = Some (msk, sc, with_trivial_spec input).
   Hypothesis fooInCtx : ∃ msk sc foo (SCP: incl sc CtxA.(SMod.scopes)),
-    alist_find CtxHdr.foo (SMod.fnsems CtxA) = Some (msk, sc, trivial_specbody foo).
+    alist_find CtxHdr.foo (SMod.fnsems CtxA) = Some (msk, sc, with_trivial_spec foo).
+
+  Local Definition main_fsp : fspec := fspec_trivial.
+  Local Definition init_cond : iProp Σ := MainA.InitCond ∗ CellioA.InitCond.
+
+  Hypothesis CtxInitCondConsistent:
+    ∀ rs, ✓ rs → (Own rs ⊢ init_cond) →
+    ∃ rs', ✓ rs' ∧ (Own rs' ⊢ init_cond ∗ CtxInitCond).
+
+  (* Apply cancellation to linked spec module *)
+  Lemma cancel_from_src :
+    refines (mod_cancel, ((init_cond ∗ CtxInitCond) ∗ main_fsp.(precond) tt tt↑ tt↑)%I) 
+            (mod_src, init_cond ∗ CtxInitCond)%I.
+  Proof. eapply cancellation; try by econs. i. iIntros "%POST". iPureIntro. des; eauto. Qed.
 
   Lemma lib_sp_incl: sp_incl CtxAS.sp sp.
   Proof.
@@ -58,61 +62,71 @@ Module CellioAll. Section CellioAll.
   Qed.
 
   (* Refinement between spec/impl of whole program (linked module) *)
-  Lemma src_tgt : refines (mod_src, init_cond) (mod_tgt, emp%I).
+  Lemma src_tgt : refines (mod_src, init_cond ∗ CtxInitCond)%I (mod_tgt, emp%I).
   Proof.
-    (* consider identical modules in src/tgt as context (CtxA, CtxA) *)
     eapply ctxr_refines.
-    rewrite -[(_, emp%I)]hmod_addc_empty_r /init_cond -!hmod_addc_assoc.
-    rewrite /mod_src /mod_tgt !add_interp_comm -!hmod_add_assoc /Ctx.
-    unseal CRIS. eapply ctxr_frameR, ctxr_cond_frameR.
+    (* consider identical modules in src/tgt as context (CtxA, CtxA) *)
+    rewrite /init_cond /mod_src /smod_src /mod_tgt.
+    rewrite !add_interp_comm.
+    
     (* solve by transitivity:
       MainI ★ CellioI ⊆ MainI ★ CellioA ⊆ MainA ★ CellioA 
     *)
-    etrans.
-    {
-      (* MainI ★ CellioA ⊆ MainA *)
-      rewrite -[(SMod.to_hmod _ MainA.Mod)](Seal.sealing_eq CRIS).
-      instantiate (1:= (MainI.t ★ (CellioA.t sp), (emp ∗ CellioA.InitCond)%I)).
-      eapply ctxr_cond_frameR, main_adequacy.
-      (* assert (XXX := @MainIA.sim). *)
-      eapply MainIA.sim.
+    etrans; cycle 1.
+    { (* CellioI ⊆ctx CellioA *)
+      ctxr_drop. ctxr_rotate. ctxr_drop.
+      eapply main_adequacy, CellioIA.sim.
       eapply lib_sp_incl.
     }
-    (* MainI ★ CellioI ⊆ MainI ★ CellioA 
-      by CellioI ⊆ctx CellioA *)
-    rewrite -[(_, emp%I)]hmod_addc_empty_r.
-    eapply ctxr_frameL, ctxr_cond_frameL, main_adequacy, CellioIA.sim.
-    eapply lib_sp_incl.
+    etrans; cycle 1.
+    { (* MainI ★ CellioA ⊆ MainA *)
+      ctxr_rotate. ctxr_drop. ctxr_rotate.
+      eapply main_adequacy, MainIA.sim.
+      eapply lib_sp_incl.
+    }
+
+    etrans; cycle 1.
+    { (* CtxI ⊆ CtxA *)
+      ctxr_rotate. ctxr_drop.
+      eapply CtxCorrect.
+    }
+    
+    rewrite /MainIAproof.MainIA.MainA /MainA.t. unseal CRIS.
+    eapply ctxr_cond_strengthen.
+    iIntros "[[? ?] ?]". iFrame.
   (*SLOW*)Qed.
 
-  Lemma cancel_tgt :
-    refines (mod_cancel, (init_cond ∗ main_fsp.(precond) tt tt↑ tt↑)%I)
+  Lemma cancel_from_tgt :
+    refines (mod_cancel, ((init_cond ∗ CtxInitCond) ∗ main_fsp.(precond) tt tt↑ tt↑)%I)
             (mod_tgt, emp%I).
   Proof.
     etrans.
-    { eapply cancel_src. }
+    { eapply cancel_from_src. }
     { eapply src_tgt. }
   Qed.
 
   Theorem behavioral_refinement :
-    ∃ target_resource, refines_mod
-      (HMod.to_mod mod_cancel (irΣ ⋅ initial_resource_own_admin))
-      (HMod.to_mod mod_tgt target_resource).
+    ∃ src_res tgt_res, refines_mod
+      (HMod.to_mod mod_cancel src_res)
+      (HMod.to_mod mod_tgt tgt_res).
   Proof.
-    move: (cancel_tgt)=>H; rewrite /refines in H; des; ss.
+    move: (cancel_from_tgt)=>H; rewrite /refines in H; des; ss.
     hexploit (H ModulesWF).
-    clear H; intros [WF H]. 
-    destruct (H (irΣ ⋅ initial_resource_own_admin)).
-    { apply irΣ_valid. }
-    { clear H. simplify_res.
-      { iDestruct "H12" as "[H2 H3]".
-        iSplitL "H2".
-        { iFrame. done. }
-        { eauto. }
-      }
-      all: solve_res.
+    clear H; intros [WF H].
+
+    assert (∃ rs, ✓ rs ∧ (Own rs ⊢ init_cond)).
+    { exists (irΣ ⋅ initial_resource_own_admin). split.
+      - apply irΣ_valid.
+      - rewrite /init_cond /MainA.InitCond /CellioA.InitCond.
+        simplify_res.
+        { iDestruct "H12" as "[H2 H3]". et. }
+        all: solve_res.
     }
-    { exists x; des; eauto. }
+    des. eapply CtxInitCondConsistent in H1; et. des.
+    
+    destruct (H rs'); et.
+    { iIntros "H". iPoseProof (H2 with "H") as "H". iFrame. et. }
+    { des. et. }
   (*SLOW*)Qed.
 End CellioAll. End CellioAll.
 (* Print Assumptions CellioAll.behavioral_refinement. *)
